theories/Lambda/ExprD.v
@@ -11,21 +11,20 @@ Set Strict Implicit.
 Export ExprDsimul.ExprDenote.
 
 Section Expr.
-  Context {typ : Type}
-          {typD : list Type -> typ -> Type}
-          {func : Type}.
-  Context {RT : RType typD}
-          {T2 : Typ2 typD PreFun.Fun}
+  Context {func : Type}.
+  Context {RT : RType}
+          {T2 : Typ2 _ PreFun.Fun}
           {RS : RSym typD func}.
 
   Instance Expr_expr : @Expr typ typD (@expr typ func) :=
-  { exprD' := fun tus tvs e t =>
-                @exprD' typ typD _ _ _ _ nil tus tvs t e
+  { exprD' := fun tus tvs e t => @exprD' _ _ _ _ nil tus tvs t e
   ; wf_Expr_acc := @wf_expr_acc typ func
   }.
 
   Instance ExprOk_expr (ts : list Type) : ExprOk Expr_expr.
-  (** TODO(gmalecha): this proof should be here **)
-  Admitted.
+  Proof.
+    constructor.
+    { admit. }
+  Qed.
 
 End Expr.
