theories/Lambda/ExprDI.v
@@ -17,23 +17,21 @@ Set Strict Implicit.
 Module Type ExprDenote.
 
   Section with_types.
-    Context {typ : Type}.
-    Context {typD : list Type -> typ -> Type}.
     Context {func : Type}.
-    Context {RType_typD : RType typD}.
-    Context {Typ2_Fun : Typ2 typD Fun}.
+    Context {RType_typD : RType}.
+    Context {Typ2_Fun : Typ2 RType_typD Fun}.
     Context {RSym_func : RSym typD func}.
 
     (** Reasoning principles **)
-    Context {RTypeOk_typD : @RTypeOk _ typD _}.
-    Context {Typ2Ok_Fun : Typ2Ok _ Typ2_Fun}.
+    Context {RTypeOk_typD : @RTypeOk _}.
+    Context {Typ2Ok_Fun : Typ2Ok Typ2_Fun}.
     Context {RSymOk_func : RSymOk RSym_func}.
 
-    Let typ_arr : typ -> typ -> typ := @typ2 _ _ _ _.
-    Let arr_match := @typ2_match _ _ _ _ .
+    Let typ_arr : typ -> typ -> typ := @typ2 _ _ _.
+    Let arr_match := @typ2_match _ _ _.
     Let typD_arr
     : forall ts a b, typD ts (typ_arr a b) = (typD ts a -> typD ts b)
-      := @typ2_cast _ _ _ _.
+      := @typ2_cast _ _ _.
 
 
     Global Instance RelDec_Rty ts : RelDec (Rty ts) :=
@@ -144,7 +142,7 @@ Module Type ExprDenote.
                                                       | None => unit
                                                     end -> typD ts _
                                        with
-                                         | eq_refl => fun x => type_weaken ts x
+                                         | eq_refl => fun x => type_weaken ts _ x
                                        end (symD f)))
                       end
       end eq_refl.
@@ -162,18 +160,18 @@ Module Type ExprDenote.
                                                     | None => unit
                                                   end -> typD ts _
                                      with
-                                       | eq_refl => fun x => type_weaken ts x
+                                       | eq_refl => fun x => type_weaken ts _ x
                                      end (symD f)))
       end eq_refl.
 
     Parameter exprD'
-    : forall {RType_typD : RType typD} {Typ2_Fun : Typ2 typD Fun}
+    : forall {Typ2_Fun : Typ2 _ Fun}
              {RSym_func : RSym typD func}
              ts (tus tvs : tenv typ) (t : typ) (e : expr typ func),
         option (OpenT ts tus tvs (typD ts t)).
 
     Axiom exprD'_respects
-    : @RTypeOk _ typD _ -> Typ2Ok _ Typ2_Fun -> RSymOk RSym_func ->
+    : @RTypeOk _ -> Typ2Ok Typ2_Fun -> RSymOk RSym_func ->
       forall ts tus tvs t t' e (pf : Rty ts t' t),
         exprD' ts tus tvs t e =
         Rcast (fun T => option (OpenT ts tus tvs T)) pf (exprD' ts tus tvs t' e).
@@ -214,7 +212,7 @@ Module Type ExprDenote.
     End typeof_expr.
 
     Axiom exprD'_Var
-    : @RTypeOk _ typD _ -> Typ2Ok _ Typ2_Fun -> RSymOk RSym_func ->
+    : @RTypeOk _ -> Typ2Ok Typ2_Fun -> RSymOk RSym_func ->
       forall ts tus tvs t v,
         exprD' ts tus tvs t (Var v) =
         bind (m := option)
@@ -227,7 +225,7 @@ Module Type ExprDenote.
                         ret (fun us vs => Rcast_val cast (get vs)))).
 
     Axiom exprD'_UVar
-    : @RTypeOk _ typD _ -> Typ2Ok _ Typ2_Fun -> RSymOk RSym_func ->
+    : @RTypeOk _ -> Typ2Ok Typ2_Fun -> RSymOk RSym_func ->
       forall ts tus tvs t u,
         exprD' ts tus tvs t (UVar u) =
         bind (m := option)
@@ -240,7 +238,7 @@ Module Type ExprDenote.
                         ret (fun us vs => Rcast_val cast (get us)))).
 
     Axiom exprD'_Inj
-    : @RTypeOk _ typD _ -> Typ2Ok _ Typ2_Fun -> RSymOk RSym_func ->
+    : @RTypeOk _ -> Typ2Ok Typ2_Fun -> RSymOk RSym_func ->
       forall ts tus tvs t s,
         exprD' ts tus tvs t (Inj s) =
         bind (m := option)
@@ -249,7 +247,7 @@ Module Type ExprDenote.
                 ret (fun _ _ => val)).
 
     Axiom exprD'_App
-    : @RTypeOk _ typD _ -> Typ2Ok _ Typ2_Fun -> RSymOk RSym_func ->
+    : @RTypeOk _ -> Typ2Ok Typ2_Fun -> RSymOk RSym_func ->
       forall ts tus tvs t f x,
         exprD' ts tus tvs t (App f x) =
         bind (m := option)
@@ -262,7 +260,7 @@ Module Type ExprDenote.
                                 ret (Open_App f x)))).
 
     Axiom exprD'_Abs
-    : @RTypeOk _ typD _ -> Typ2Ok _ Typ2_Fun -> RSymOk RSym_func ->
+    : @RTypeOk _ -> Typ2Ok Typ2_Fun -> RSymOk RSym_func ->
       forall ts tus tvs t t' e,
         exprD' ts tus tvs t (Abs t' e) =
         arr_match (fun T => option (OpenT ts tus tvs T)) ts t
@@ -284,26 +282,24 @@ End ExprDenote.
 Module Type ExprFacts (ED : ExprDenote).
 
   Section with_types.
-    Context {typ : Type}.
-    Context {typD : list Type -> typ -> Type}.
-    Context {RType_typD : RType typD}.
-    Context {Typ2_Fun : Typ2 typD Fun}.
+    Context {RType_typD : RType}.
+    Context {Typ2_Fun : Typ2 _ Fun}.
     Context {func : Type}.
     Context {RSym_func : RSym typD func}.
 
     (** Reasoning principles **)
-    Context {RTypeOk_typD : @RTypeOk _ typD _}.
-    Context {Typ2Ok_Fun : Typ2Ok _ Typ2_Fun}.
+    Context {RTypeOk_typD : @RTypeOk _}.
+    Context {Typ2Ok_Fun : Typ2Ok Typ2_Fun}.
     Context {RSymOk_func : RSymOk RSym_func}.
 
     Axiom typeof_expr_weaken
-    : @RTypeOk _ typD _ -> Typ2Ok _ Typ2_Fun -> RSymOk RSym_func ->
+    : @RTypeOk _ -> Typ2Ok Typ2_Fun -> RSymOk RSym_func ->
       forall ts tus tvs e t tus' tvs',
         ED.typeof_expr ts tus tvs e = Some t ->
         ED.typeof_expr ts (tus ++ tus') (tvs ++ tvs') e = Some t.
 
     Axiom exprD'_weaken
-    : @RTypeOk _ typD _ -> Typ2Ok _ Typ2_Fun -> RSymOk RSym_func ->
+    : @RTypeOk _ -> Typ2Ok Typ2_Fun -> RSymOk RSym_func ->
       forall ts tus tvs (e : expr typ func) t val tus' tvs',
         ED.exprD' ts tus tvs t e = Some val ->
         exists val',
@@ -312,13 +308,13 @@ Module Type ExprFacts (ED : ExprDenote).
             val us vs = val' (hlist_app us us') (hlist_app vs vs').
 
     Axiom exprD'_type_cast
-    : @RTypeOk _ typD _ -> Typ2Ok _ Typ2_Fun -> RSymOk RSym_func ->
+    : @RTypeOk _ -> Typ2Ok Typ2_Fun -> RSymOk RSym_func ->
       forall ts tus tvs e t,
         ED.exprD' ts tus tvs t e =
         match ED.typeof_expr ts tus tvs e with
           | None => None
           | Some t' =>
-            match @type_cast _ typD _ ts t' t with
+            match @type_cast _ ts t' t with
               | None => None
               | Some cast =>
                 match ED.exprD' ts tus tvs t' e with
@@ -330,7 +326,7 @@ Module Type ExprFacts (ED : ExprDenote).
         end.
 
     Axiom typeof_expr_exprD'
-    : @RTypeOk _ typD _ -> Typ2Ok _ Typ2_Fun -> RSymOk RSym_func ->
+    : @RTypeOk _ -> Typ2Ok Typ2_Fun -> RSymOk RSym_func ->
       forall ts tus tvs e t,
         ED.typeof_expr ts tus tvs e = Some t ->
         exists val,
